restored foldl version of proof for tesseract.

src/specs/tesseract.fst
@@ -42,52 +42,53 @@ module Tesseract.Specs.Tesseract
       (step_kind_t: Type) 
       = Seq.seq_g (effect_g region_t state_t step_kind_t)
 
-   type _is_tesseract_safe: 
+   val _domain: 
+      #region_t: Type 
+      -> #state_t: Type 
+      -> #step_kind_t: Type 
+      -> _tesseract_g region_t state_t step_kind_t
+      -> Tot (option (Set.set_g region_t))
+   let _domain
+      (region_t: Type)
+      (state_t: Type)
+      (step_kind_t: Type)
+      _tess
+      = let on_fold 
+         = (fun accum ffct
+            -> match accum with
+                  | None ->
+                     // an unsafe tesseract continues to be unsafe.
+                     None
+                  | Some set ->
+                     // examine the next effect in the sequence.
+                     (match ffct with
+                        | Spawn region _ _ ->
+                           // if we're looking at a spawn effect associated with a region, that region must not have already set.
+                           if Set.is_mem set region then
+                              None
+                           // otherwise, note that we have encountered it.
+                           else
+                              Some (Set.add set region)
+                        | Step region _ ->
+                           // a step effect associated with a given region must be in our set of set regions.
+                           if Set.is_mem set region then
+                              accum
+                           else
+                              None))
+         in (Seq.foldl on_fold (Some Set.empty) _tess)
+
+   val _is_tesseract_safe: 
       #region_t: Type 
       -> #state_t: Type 
       -> #step_kind_t: Type 
       -> _tesseract_g region_t state_t step_kind_t 
-      -> Type
-      = fun
-         (region_t: Type)
-         (state_t: Type)
-         (step_kind_t: Type)
-         (_tess: _tesseract_g region_t state_t step_kind_t)
-         -> // empty sequences are safe.
-            (0 = (Seq.length _tess))
-            \/ // only one spawn effect per region exists.
-               ((forall i j.
-                  (0 <= i)
-                  && (i < Seq.length _tess)
-                  && (is_Spawn (Seq.nth _tess i))
-                  && (0 <= j)
-                  && (j < Seq.length _tess)
-                  && (is_Spawn (Seq.nth _tess j))
-                  ==> ((Spawn.region (Seq.nth _tess i)) = (Spawn.region (Seq.nth _tess j))))
-               /\ // if only one effect exists in the sequence, then we're good if it's a spawn event.
-                  (1 = (Seq.length _tess) ==> is_Spawn (Seq.nth _tess 0))
-                  \/ // otherwise, any step effects for a given region are preceeded by a matching regional spawn effect.
-                     ((forall i.
-                        (0 < i)
-                        && (i < Seq.length _tess)
-                        && (is_Step (Seq.nth _tess i))
-                        ==> (exists j.
-                              (0 <= j)
-                              && (j < i)
-                              && (j < (Seq.length _tess - 1)) // todo: seems that a trasitivity lemma for < would be useful here.
-                              && (is_Spawn (Seq.nth _tess j))
-                              && ((Step.region (Seq.nth _tess i)) = (Spawn.region (Seq.nth _tess j))))) 
-                     /\ // also, spawn effects cannot be preceeded by matching step effects.
-                        (exists i.
-                           (0 < i)
-                           && (i < Seq.length _tess)
-                           && (is_Spawn (Seq.nth _tess i))
-                           ==> (forall j.
-                                 (0 <= j)
-                                 && (j < i)
-                                 && (j < (Seq.length _tess - 1)) // todo: transitive <?
-                                 && (is_Step (Seq.nth _tess j))
-                                 && ((Spawn.region (Seq.nth _tess i)) <> (Step.region (Seq.nth _tess j)))))))
+      -> Tot bool
+   let _is_tesseract_safe 
+      (region_t: Type)
+      (state_t: Type)
+      (step_kind_t: Type)
+      (_tess: _tesseract_g region_t state_t step_kind_t)
+      = is_Some (_domain _tess)
 
    type tesseract_g 
       (region_t: Type) 
@@ -121,19 +122,9 @@ module Tesseract.Specs.Tesseract
       (state_t: Type)
       (step_kind_t: Type)
       tess
-      = let on_fold 
-         = (fun (spawned: Set.set_g region_t) (ffct: effect_g region_t state_t step_kind_t)
-            -> // examine the next effect in the sequence.
-               match ffct with
-                  | Spawn region _ _ ->
-                     // the spawn effect always introduces new regions and shouldn't already be a member of the spawned set.
-                     assert (not (Set.is_mem spawned region));
-                     Set.add spawned region
-                  | Step region _ ->
-                     // a step effect associated with a given region must be in our set of spawned regions.
-                     assert (Set.is_mem spawned region);
-                     spawned)
-         in (Seq.foldl on_fold Set.empty tess)
+      = match _domain tess with
+         | Some d ->
+            d
 
    val is_mem:
       #region_t: Type
